\JGWitem{Nov 2001, \#38}
For a triple decrement model:
\begin{enumerate}
\item
\begin{tabular}[b]{cccc}
   $x$  & $q_{x}^{'(1)}$ & $q_{x}^{'(2)}$ & $q_{x}^{'(3)}$ \\ \hline
    63  & 0.02000           & 0.03000           &    0.25000 \\
    64 & 0.02500            & 0.03500           & 0.20000 \\
    65 & 0.03000            & 0.04000             & 0.15000
\end{tabular}
\item  $q_{65}^{(1)} = 0.02716$
\item  Each decrement has a constant force over each year of age.
\end{enumerate}
Calculate $\prepostsubsup{2}{q}{64}{(1)}$
\showMC{\begin{description}
\item[(A)] 0.04182
\item[(B)] 0.04248
\item[(C)] 0.04314
\item[(D)] 0.04480
\item[(E)] 0.04546
\end{description}}
\showsol{\bsoln
\showMC{\underline{ANS: (B)}}

Following Example 13.2(c) in the text we note that
\be \label{C3Nov2001_38.1}
   \prepostsubsup{2}{q}{64}{(1)} = q_{64}^{(1)} + p_{64}^{(\tau)}\cdot q_{65}^{(1)}.
\ee

In general, \dsy{q_{x}^{(i)} = \int_0^1 \prepostsubsup{t}{p}{x}{(\tau)}\,\mu_{x+t}^{(i)}\,dt}, and
in the special case of constant HRF for $t=\in[0,1]$ this simplifies to
\[
    q_{x}^{(i)} = \frac{\log(p_x^{'(i)})}{\log(p_x^{'(\tau)})}q_x^{(\tau)}
\]
(see ``Case B1'' in the big table on page 352).

So (\ref{C3Nov2001_38.1}) becomes
\[
  \prepostsubsup{2}{q}{64}{(1)} =  \frac{\log(p_{64}^{'(i)})}{\log(p_{64}^{'(\tau)})}q_{64}^{(\tau)}
    + p_{64}^{(\tau)}\cdot \frac{\log(p_{65}^{'(i)})}{\log(p_{65}^{'(\tau)})}q_{65}^{(\tau)}
\]
We have all the $p_x^{'(i)}$'s, and we also need:
\bears
    p_{64}^{(\tau)} &=& = \left(p_{64}^{'(1)}\right)\left(p_{64}^{'(2)}\right)\left(p_{64}^{'(3)}\right)
              \left(1-q_{64}^{'(1)}\right)\left(1-q_{64}^{'(2)}\right)\left(1-q_{64}^{'(3)}\right) = 0.7527, \\
  q_{64}^{(\tau)} &=& = 1- 0.7527 = 0.2473, \\
  p_{65}^{(\tau)} &=& = \left(p_{65}^{'(1)}\right)\left(p_{65}^{'(2)}\right)\left(p_{65}^{'(3)}\right)
            \left(1-q_{65}^{'(1)}\right)\left(1-q_{65}^{'(2)}\right)\left(1-q_{65}^{'(3)}\right) = 0.79152, \\
 q_{65}^{(\tau)} &=& = 1- 0.79152 = 0.20848
\eears
So  \ldots
\esoln}
